fstar/code/arch/x64/X64.Vale.Xmms.fsti
@@ -3,14 +3,13 @@ module X64.Vale.Xmms
 
 open Prop_s
 open X64.Machine_s
-unfold let quad32 = Types_s.quad32
 
-type t = xmm -> quad32
+type t = xmms_t
 
 val equal (xmms1:t) (xmms2:t) : prop0
 
 val lemma_equal_intro (xmms1:t) (xmms2:t) : Lemma
-  (requires forall x. xmms1 x == xmms2 x)
+  (requires forall (x:xmm). xmms1 x == xmms2 x)
   (ensures equal xmms1 xmms2)
   [SMTPat (equal xmms1 xmms2)]
 
